Introduce na_inv_wsat

nola/examples/logic/iris.v
@@ -7,12 +7,6 @@ From nola.examples.heap_lang Require Export definitions.
 
 (** ** Iris resources *)
 
-(** Data for invariant *)
-Variant nInvd : Type :=
-| (* usual *) nInvd_u (P : nPropS (;ᵞ))
-| (* non-atomic *) nInvd_na
-    (p : na_inv_pool_name) (i : positive) (P : nPropS (;ᵞ)).
-
 (** Agreement *)
 Class agreeG A Σ := agree_inG :: inG Σ (agreeR (leibnizO A)).
 Definition agreeΣ A : gFunctors := GFunctor (agreeR (leibnizO A)).
@@ -21,29 +15,14 @@ Proof. solve_inG. Qed.
 
 (** [nintpGS]: Iris resource *)
 Class nintpGS Σ := NintpGS {
-  nintpGS_agreeG :: agreeG (nPropL (;ᵞ)) Σ;
-  nintpGS_ninvGS :: ninvGS nInvd Σ;
-  nintpGS_na_invG :: na_invG Σ;
-  nintpGS_cinvG :: cinvG Σ;
-  nintpGS_heapGS :: heapGS_gen HasNoLc Σ;
+  nintpGS_agree :: agreeG (nPropL (;ᵞ)) Σ;
+  nintpGS_ninv :: ninvGS (nPropS (;ᵞ)) Σ;
+  nintpGS_na_ninv :: na_ninvGS (nPropS (;ᵞ)) Σ;
+  nintpGS_na_inv :: na_invG Σ;
+  nintpGS_cinv :: cinvG Σ;
+  nintpGS_heap :: heapGS_gen HasNoLc Σ;
 }.
 Arguments NintpGS {_} _ _ _ _ _.
-
-Section nInvd_intp.
-  Context `{!nintpGS Σ}.
-
-  (** Interpret [nInvd] *)
-  Definition nInvd_intp (intp : nPropS (;ᵞ) -d> iProp Σ) : nInvd -d> iProp Σ :=
-    λ Px, match Px with
-    | nInvd_u P => intp P
-    | nInvd_na p i P => na_body p i (intp P)
-    end.
-  #[export] Instance nInvd_intp_ne : NonExpansive nInvd_intp.
-  Proof. solve_proper. Qed.
-End nInvd_intp.
-
-(** [inv_wsat] for [nInvd] *)
-Notation inv_wsat' intp := (inv_wsat (nInvd_intp intp)).
 
 (** ** Derivability structure *)
 
@@ -76,9 +55,9 @@ Section iris.
   (** [na_ninv]: [na_ninv] in the accessor style *)
   Definition na_ninv_def (δ : nderiv_ty Σ)
     (p : na_inv_pool_name) (N : namespace) (P : nPropL (;ᵞ)) : iProp Σ :=
-    □ ⸨ ∀ E F, ⌜↑N ⊆ E⌝ → ⌜↑N ⊆ F⌝ → n_na_own p F =[n_inv_wsat]{E}=∗
-          P ∗ n_na_own p (F∖↑N) ∗
-          (P -∗ n_na_own p (F∖↑N) =[n_inv_wsat]{E}=∗ n_na_own p F) ⸩(δ).
+    □ ⸨ ∀ E F, ⌜↑N ⊆ E⌝ → ⌜↑N ⊆ F⌝ → n_na_own p F =[n_na_inv_wsat]{E}=∗
+          n_na_own p (F∖↑N) ∗ P ∗
+          (n_na_own p (F∖↑N) -∗ P =[n_na_inv_wsat]{E}=∗ n_na_own p F) ⸩(δ).
   Definition na_ninv_aux : seal na_ninv_def. Proof. by eexists. Qed.
   Definition na_ninv := na_ninv_aux.(unseal).
   Lemma na_ninv_unseal : na_ninv = na_ninv_def. Proof. exact: seal_eq. Qed.
