nola/iris/na_inv.v
@@ -5,27 +5,41 @@ From iris.base_logic Require Export lib.na_invariants.
 From iris.algebra Require Import gset coPset.
 From iris.proofmode Require Import proofmode.
 
+Implicit Type PROP : Type.
+Implicit Type (p : na_inv_pool_name) (i : positive).
+
+#[projections(primitive)]
+Record na_prop PROP := NaProp {
+  na_prop_p : na_inv_pool_name;
+  na_prop_i : positive;
+  na_prop_P : PROP;
+}.
+Arguments NaProp {_} _ _ _.
+Add Printing Constructor na_prop.
+
+Class na_ninvGS PROP Σ := na_ninvGS_in : ninvGS (na_prop PROP) Σ.
+Local Existing Instance na_ninvGS_in.
+Class na_ninvGpreS PROP Σ := na_ninvGpreS_in : ninvGpreS (na_prop PROP) Σ.
+Local Existing Instance na_ninvGpreS_in.
+Definition na_ninvΣ PROP : gFunctors := ninvΣ (na_prop PROP).
+#[export] Instance subG_na_ninvΣ `{!subG (na_ninvΣ PROP) Σ} :
+  na_ninvGpreS PROP Σ.
+Proof. solve_inG. Qed.
+
 Section na_ninv.
-  Context `{!invGS_gen hlc Σ, !na_invG Σ}.
+  Context `{!na_ninvGS PROP Σ, !invGS_gen hlc Σ, !na_invG Σ}.
+  Implicit Type intp : PROP -d> iProp Σ.
   Local Existing Instance na_inv_inG.
 
-  (** Access lock of an non-atomic invariant *)
-  Definition na_lock (p : na_inv_pool_name) (i : positive) : iProp Σ :=
-    own p (ε, GSet {[i]}).
-
-  (** What to be put in an non-atomic invariant *)
-  Definition na_body
-    (p : na_inv_pool_name) (i : positive) (P : iProp Σ) : iProp Σ :=
-    P ∗ na_lock p i ∨ na_own p {[i]}.
-  #[export] Instance na_body_ne {p i} : NonExpansive (na_body p i).
-  Proof. solve_proper. Qed.
+  (** Access l of an non-atomic invariant *)
+  Local Definition na_lock p i : iProp Σ := own p (ε, GSet {[i]}).
 
   (** Allocate [na_lock] *)
-  Lemma na_lock_alloc {p N} :
+  Local Lemma na_lock_alloc {p N} :
     ⊢ |==> ∃ i, ⌜i ∈ (↑N:coPset)⌝ ∧ na_lock p i.
   Proof.
     iMod (own_unit (prodUR coPset_disjUR (gset_disjUR positive)) p) as "ε".
-    iMod (own_updateP with "ε") as ([m1 m2]) "[%cond lock]".
+    iMod (own_updateP with "ε") as ([m1 m2]) "[%cond l]".
     { apply prod_updateP'.
       - apply cmra_updateP_id, (reflexivity (R:=eq)).
       - apply (gset_disj_alloc_empty_updateP_strong' (.∈ (↑N:coPset)))=> ?.
@@ -33,19 +47,91 @@ Section na_ninv.
     move: cond=>/=[<-[i[->?]]]. iModIntro. iExists i. by iSplit.
   Qed.
 
+  (** What to be put in a non-atomic invariant *)
+  Local Definition na_body p i (P : iProp Σ) : iProp Σ :=
+    P ∗ na_lock p i ∨ na_own p {[i]}.
+
   (** Access [P] from [na_body] *)
-  Lemma na_body_acc {p i N E P} : i ∈ (↑N:coPset) → ↑N ⊆ E →
-    na_body p i P -∗ na_own p E -∗
-      na_body p i P ∗ P ∗ na_own p (E∖↑N) ∗
-      (na_body p i P -∗ P -∗ na_own p (E∖↑N) -∗ na_body p i P ∗ na_own p E).
+  Local Lemma na_body_acc {p i N E P} : i ∈ (↑N:coPset) → ↑N ⊆ E →
+    na_own p E -∗ na_body p i P -∗
+      na_own p (E∖↑N) ∗ na_body p i P ∗ P ∗
+      (na_own p (E∖↑N) -∗ na_body p i P -∗ P -∗ na_body p i P ∗ na_own p E).
   Proof.
-    iIntros (??) "[[$ lock]|i] E"; last first.
+    iIntros (??) "E [[$ l]|i]"; last first.
     { iDestruct (na_own_disjoint with "i E") as %?. set_solver. }
     rewrite [E as X in na_own p X](union_difference_L (↑N) E); [|done].
     rewrite [X in (X ∪ _)](union_difference_L {[i]} (↑N)) ?na_own_union;
       [|set_solver..].
-    iDestruct "E" as "[[$$] $]". iIntros "[[_ lock']|i] P $".
-    - iCombine "lock lock'" gives %[_ Hval%gset_disj_valid_op]. set_solver.
+    iDestruct "E" as "[[$$] $]". iIntros "$ [[_ l']|i] P".
+    - iCombine "l l'" gives %[_ Hval%gset_disj_valid_op]. set_solver.
     - iSplitR "i"; [|done]. iLeft. iFrame.
   Qed.
+
+  (** Token for a non-atomic invariant *)
+  Local Definition na_inv_tok_def p N (P : PROP) : iProp Σ :=
+    ∃ i, ⌜i ∈ (↑N:coPset)⌝ ∗ inv_tok N (NaProp p i P).
+  Local Lemma na_inv_tok_aux : seal na_inv_tok_def. Proof. by eexists. Qed.
+  Definition na_inv_tok := na_inv_tok_aux.(unseal).
+  Local Lemma na_inv_tok_unseal : na_inv_tok = na_inv_tok_def.
+  Proof. exact: seal_eq. Qed.
+
+  (** [na_inv_tok] is persistent and timeless *)
+  #[export] Instance na_inv_tok_persistent {p N P} :
+    Persistent (na_inv_tok p N P).
+  Proof. rewrite na_inv_tok_unseal. exact _. Qed.
+  #[export] Instance na_inv_tok_timeless {p N P} : Timeless (na_inv_tok p N P).
+  Proof. rewrite na_inv_tok_unseal. exact _. Qed.
+
+  (** World satisfaction for non-atomic invariants *)
+  Local Definition na_inv_wsat_def intp : iProp Σ :=
+    inv_wsat (λ '(NaProp p i P), na_body p i (intp P)).
+  Local Lemma na_inv_wsat_aux : seal na_inv_wsat_def. Proof. by eexists. Qed.
+  Definition na_inv_wsat := na_inv_wsat_aux.(unseal).
+  Local Lemma na_inv_wsat_unseal : na_inv_wsat = na_inv_wsat_def.
+  Proof. exact: seal_eq. Qed.
+
+  (** [na_inv_wsat] is non-expansive *)
+  #[export] Instance na_inv_wsat_ne : NonExpansive na_inv_wsat.
+  Proof.
+    rewrite na_inv_wsat_unseal /na_inv_wsat_def=> ????. f_equiv. case=> >.
+    solve_proper.
+  Qed.
+  #[export] Instance na_inv_wsat_proper : Proper ((≡) ==> (≡)) inv_wsat.
+  Proof. apply ne_proper, _. Qed.
+
+  (** Allocate [na_inv_tok] *)
+  Lemma na_inv_tok_alloc_rec {intp} P p N :
+    (na_inv_tok p N P -∗ intp P) =[na_inv_wsat intp]=∗ na_inv_tok p N P.
+  Proof.
+    rewrite na_inv_tok_unseal na_inv_wsat_unseal.
+    iIntros "→P". iMod na_lock_alloc as (i ?) "l".
+    iMod (inv_tok_alloc_rec with "[→P l]"); last first.
+    { iModIntro. iExists _. by iSplit. }
+    iIntros "i". iLeft. iFrame "l". iApply "→P". iExists _. by iSplit.
+  Qed.
+  Lemma na_inv_tok_alloc {intp} P p N :
+    intp P =[na_inv_wsat intp]=∗ na_inv_tok p N P.
+  Proof. iIntros "?". iApply na_inv_tok_alloc_rec. by iIntros. Qed.
+
+  (** Access [na_inv_tok] *)
+  Lemma na_inv_tok_acc {intp p N E F P} : ↑N ⊆ E → ↑N ⊆ F →
+    na_own p F -∗ na_inv_tok p N P =[na_inv_wsat intp]{E}=∗
+      na_own p (F∖↑N) ∗ intp P ∗
+      (na_own p (F∖↑N) -∗ intp P =[na_inv_wsat intp]{E}=∗ na_own p F).
+  Proof.
+    rewrite na_inv_tok_unseal na_inv_wsat_unseal=> ??. iIntros "F [%i[% #i]]".
+    iMod (inv_tok_acc with "i") as "[bd cl]"; [done|].
+    iDestruct (na_body_acc with "F bd") as "[$[bd[$ →bdF]]]"; [done..|].
+    iMod ("cl" with "bd") as "_". iIntros "!> F∖N P".
+    iMod (inv_tok_acc with "i") as "[bd cl]"; [done|].
+    iDestruct ("→bdF" with "F∖N bd P") as "[bd $]". by iApply "cl".
+  Qed.
 End na_ninv.
+
+(** Allocate [na_inv_wsat] *)
+Lemma na_inv_wsat_alloc `{!na_ninvGpreS PROP Σ, !invGS_gen hlc Σ, !na_invG Σ} :
+  ⊢ |==> ∃ _ : na_ninvGS PROP Σ, ∀ intp, na_inv_wsat intp.
+Proof.
+  iMod inv_wsat_alloc as (?) "W". iModIntro. iExists _. iIntros (?).
+  rewrite na_inv_wsat_unseal. iApply "W".
+Qed.
