nola/examples/logic/adequacy.v
@@ -5,35 +5,41 @@ From nola.examples.heap_lang Require Export adequacy total_adequacy.
 
 (** Precursor of [nintpGS] *)
 Class nintpGpreS Σ := NintpGpreS {
-  nintpGpreS_agreeG :: agreeG (nPropL (;ᵞ)) Σ;
-  nintpGpreS_ninvGpreS :: ninvGpreS nInvd Σ;
-  nintpGpreS_na_invG :: na_invG Σ;
-  nintpGpreS_cinvG :: cinvG Σ;
-  nintpGpreS_heapGpreS :: heapGpreS Σ;
+  nintpGpreS_agree :: agreeG (nPropL (;ᵞ)) Σ;
+  nintpGpreS_ninv :: ninvGpreS (nPropS (;ᵞ)) Σ;
+  nintpGpreS_na_ninv :: na_ninvGpreS (nPropS (;ᵞ)) Σ;
+  nintpGpreS_na_inv :: na_invG Σ;
+  nintpGpreS_cinv :: cinvG Σ;
+  nintpGpreS_heap :: heapGpreS Σ;
 }.
 
 (** [gFunctors] for [nintpGpreS] *)
 Definition nintpΣ : gFunctors :=
-  #[agreeΣ (nPropL (;ᵞ)); ninvΣ nInvd; na_invΣ; cinvΣ; heapΣ].
+  #[agreeΣ (nPropL (;ᵞ)); ninvΣ (nPropS (;ᵞ)); na_ninvΣ (nPropS (;ᵞ));
+    na_invΣ; cinvΣ; heapΣ].
 #[export] Instance subG_nintpGpreS `{!subG nintpΣ Σ} : nintpGpreS Σ.
 Proof. solve_inG. Qed.
 
 (** Adequacy of [wp] over [inv_wsatd] *)
 Lemma wp_n_adequacy `{!nintpGpreS Σ} {s e σ φ} :
-  (∀ `{!nintpGS Σ}, inv_heap_inv -∗ WP[inv_wsatd] e @ s; ⊤ {{ v, ⌜φ v⌝ }}) →
+  (∀ `{!nintpGS Σ}, inv_heap_inv -∗
+    WP[inv_wsatd ∗ na_inv_wsatd] e @ s; ⊤ {{ v, ⌜φ v⌝ }}) →
   adequate s e σ (λ v _, φ v).
 Proof.
   move=> towp. apply (heap_adequacy Σ HasNoLc)=> ?.
-  iMod inv_wsat_alloc as (?) "?". iModIntro. iExists inv_wsatd.
-  iSplitL; [done|]. iApply (towp (NintpGS _ _ _ _ _)).
+  iMod inv_wsat_alloc as (?) "W". iMod na_inv_wsat_alloc as (?) "W'". iModIntro.
+  iExists (inv_wsatd ∗ na_inv_wsatd)%I. iSplitL; [by iSplitL "W"|].
+  iApply (towp (NintpGS _ _ _ _ _ _)).
 Qed.
 
 (** Adequacy of [twp] over [inv_wsatd] *)
 Lemma twp_n_adequacy `{!nintpGpreS Σ} {s e σ φ} :
-  (∀ `{!nintpGS Σ}, inv_heap_inv -∗ WP[inv_wsatd] e @ s; ⊤ [{ v, ⌜φ v⌝ }]) →
+  (∀ `{!nintpGS Σ}, inv_heap_inv -∗
+    WP[inv_wsatd ∗ na_inv_wsatd] e @ s; ⊤ [{ v, ⌜φ v⌝ }]) →
   sn erased_step ([e], σ).
 Proof.
   move=> totwp. apply (heap_total Σ s _ _ φ)=> ?.
-  iMod inv_wsat_alloc as (?) "?". iModIntro. iExists inv_wsatd.
-  iSplitL; [done|]. iApply (totwp (NintpGS _ _ _ _ _)).
+  iMod inv_wsat_alloc as (?) "W". iMod na_inv_wsat_alloc as (?) "W'". iModIntro.
+  iExists (inv_wsatd ∗ na_inv_wsatd)%I. iSplitL; [by iSplitL "W"|].
+  iApply (totwp (NintpGS _ _ _ _ _ _)).
 Qed.
