nola/examples/logic/inv.v
@@ -20,7 +20,7 @@ Section lemmas.
 
   (** Turn [inv_tok] into [ninv] *)
   Local Lemma inv_tok_ninv {P : nPropS _} {N} :
-    inv_tok N (nInvd_u P) ⊢ ninv δ N (↑ˡ P).
+    inv_tok N P ⊢ ninv δ N (↑ˡ P).
   Proof.
     rewrite ninv_unseal. iIntros "#NP !>". iApply (derivy_intro (δ:=δ))=>/=.
     iIntros (?????). rewrite -nintpS_nintp_nlarge.
@@ -30,9 +30,8 @@ Section lemmas.
   Lemma ninv_alloc_rec (P : nPropS _) N :
     (ninv δ N (↑ˡ P) -∗ ⟦ P ⟧(δ)) =[inv_wsat' δ]=∗ ninv δ N (↑ˡ P).
   Proof.
-    rewrite -inv_tok_ninv. iIntros "→P".
-    iApply (inv_tok_alloc_rec (nInvd_u P) with "[→P]"). iIntros "NP".
-    rewrite/= nintpS_nintp. by iApply "→P".
+    rewrite -inv_tok_ninv. iIntros "→P". iApply (inv_tok_alloc_rec with "[→P]").
+    iIntros "NP". rewrite nintpS_nintp. by iApply "→P".
   Qed.
   Lemma ninv_alloc (P : nPropS _) N :
     ⟦ P ⟧(δ) =[inv_wsat' δ]=∗ ninv δ N (↑ˡ P).
