nola/examples/logic/na_inv.v
@@ -9,11 +9,11 @@ Section lemmas.
 
   (** Access [na_ninv] *)
   Lemma na_ninv_acc {p N P E F} : ↑N ⊆ E → ↑N ⊆ F →
-    na_ninvd p N P -∗ na_own p F =[inv_wsatd]{E}=∗
-      ⟦ P ⟧ ∗ na_own p (F∖↑N) ∗
-      (⟦ P ⟧ -∗ na_own p (F∖↑N) =[inv_wsatd]{E}=∗ na_own p F).
+    na_own p F -∗ na_ninvd p N P =[na_inv_wsatd]{E}=∗
+      na_own p (F∖↑N) ∗ ⟦ P ⟧ ∗
+      (na_own p (F∖↑N) -∗ ⟦ P ⟧ =[na_inv_wsatd]{E}=∗ na_own p F).
   Proof.
-    rewrite na_ninv_unseal. iIntros (NE NF) "#∝P F".
+    rewrite na_ninv_unseal. iIntros (NE NF) "F #∝P".
     iDestruct nderiv_sound as "→".
     iDestruct ("→" with "∝P") as "/={∝P}∝P".
     iApply ("∝P" $! _ _ NE NF with "F").
@@ -22,31 +22,24 @@ Section lemmas.
   Context `{!nderivy ih δ}.
 
   (** Turn [na_ninv] into [na_ninv] *)
-  Local Lemma na_inv_tok_ninv {P : nPropS _} {i p N} : i ∈ (↑N:coPset) →
-    inv_tok N (nInvd_na p i P) ⊢ na_ninv (Σ:=Σ) δ p N (↑ˡ P).
+  Local Lemma na_inv_tok_ninv {P : nPropS _} {p N} :
+    na_inv_tok p N P ⊢ na_ninv (Σ:=Σ) δ p N (↑ˡ P).
   Proof.
-    rewrite na_ninv_unseal. iIntros (jN) "#NP !>".
-    iApply (derivy_intro (δ:=δ))=>/=.
-    iIntros (??? E F NE NF) "F". rewrite -nintpS_nintp_nlarge.
-    iMod (inv_tok_acc NE with "NP") as "/=[bd bd→]".
-    iDestruct (na_body_acc with "bd F") as "(bd &$&$& P→)"; [done..|].
-    iMod ("bd→" with "bd") as "_". iIntros "!> P F∖N".
-    iMod (inv_tok_acc NE with "NP") as "/=[bd bd→]".
-    iDestruct ("P→" with "bd P F∖N") as "[bd $]".
-    by iMod ("bd→" with "bd") as "_".
+    rewrite na_ninv_unseal. iIntros "#NP !>". iApply (derivy_intro (δ:=δ))=>/=.
+    iIntros (???????) "F". rewrite -nintpS_nintp_nlarge.
+    by iApply (na_inv_tok_acc with "F NP").
   Qed.
   (** Allocate [na_ninv] *)
   Lemma na_ninv_alloc_rec (P : nPropS _) p N :
-    (na_ninv δ p N (↑ˡ P) -∗ ⟦ P ⟧(δ)) =[inv_wsat' δ]=∗
+    (na_ninv δ p N (↑ˡ P) -∗ ⟦ P ⟧(δ)) =[na_inv_wsat' δ]=∗
       na_ninv δ p N (↑ˡ P).
   Proof.
-    iIntros "→P". iMod na_lock_alloc as (i) "[% lock]".
-    rewrite -na_inv_tok_ninv; [|done].
-    iApply (inv_tok_alloc_rec (nInvd_na p i P) with "[→P lock]").
-    iIntros "/=NP". iLeft. iFrame "lock". rewrite nintpS_nintp. by iApply "→P".
+    rewrite -na_inv_tok_ninv. iIntros "→P".
+    iApply (na_inv_tok_alloc_rec with "[→P]"). iIntros "NP".
+    rewrite nintpS_nintp. by iApply "→P".
   Qed.
   Lemma na_ninv_alloc (P : nPropS _) p N :
-    ⟦ P ⟧(δ) =[inv_wsat' δ]=∗ na_ninv δ p N (↑ˡ P).
+    ⟦ P ⟧(δ) =[na_inv_wsat' δ]=∗ na_ninv δ p N (↑ˡ P).
   Proof.
     iIntros "P". iApply (na_ninv_alloc_rec with "[P]"). by iIntros.
   Qed.
@@ -58,11 +51,11 @@ Section lemmas.
     rewrite na_ninv_unseal. iIntros "#PQP #∝P !>".
     iApply (derivy_map2 with "[] PQP ∝P")=>/=.
     iIntros (???) "/= {PQP}PQP {∝P}∝P". iIntros (E F NE NF) "F".
-    iMod ("∝P" $! E F NE NF with "F") as "(P &$& P→)".
+    iMod ("∝P" $! E F NE NF with "F") as "[$[P P→]]".
     iMod (fupd_mask_subseteq ∅) as "→E∖N"; [set_solver|].
-    iMod ("PQP" with "P") as "($& QP)". iMod "→E∖N" as "_". iIntros "!> Q".
+    iMod ("PQP" with "P") as "[$ QP]". iMod "→E∖N" as "_". iIntros "!> F∖N Q".
     iMod (fupd_mask_subseteq ∅) as "→E∖N"; [set_solver|].
-    iMod ("QP" with "Q") as "P". iMod "→E∖N" as "_". iApply ("P→" with "P").
+    iMod ("QP" with "Q") as "P". iMod "→E∖N" as "_". iApply ("P→" with "F∖N P").
   Qed.
   Lemma na_ninv_split {p N P Q} :
     na_ninv δ p N (P ∗ Q) ⊢ na_ninv δ p N P ∗ na_ninv δ p N Q.
@@ -91,11 +84,11 @@ Section lemmas.
     rewrite na_ninv_unseal. iIntros (??) "#NP #N'Q !>".
     iApply (derivy_map2 (δ:=δ) with "[] NP N'Q")=>/=.
     iIntros (???) "{NP}NP {N'Q}N'Q". iIntros (? F ??) "F".
-    iMod ("NP" with "[%] [%] F") as "($& F∖N & P→)"; [set_solver..|].
-    iMod ("N'Q" with "[%] [%] F∖N") as "($& F∖NN' & Q→)"; [set_solver..|].
+    iMod ("NP" with "[%] [%] F") as "[F∖N[$ P→]]"; [set_solver..|].
+    iMod ("N'Q" with "[%] [%] F∖N") as "[F∖NN'[$ Q→]]"; [set_solver..|].
     iDestruct (na_own_acc with "F∖NN'") as "[$ F∖N''→]"; [set_solver|].
-    iApply fupdw_mask_intro; [set_solver|]. iIntros "cl [P Q] F∖N''".
+    iApply fupdw_mask_intro; [set_solver|]. iIntros "cl F∖N'' [P Q]".
     iMod "cl" as "_". iDestruct ("F∖N''→" with "F∖N''") as "F∖NN'".
-    iMod ("Q→" with "Q F∖NN'") as "F∖N". iApply ("P→" with "P F∖N").
+    iMod ("Q→" with "F∖NN' Q") as "F∖N". iApply ("P→" with "F∖N P").
   Qed.
 End lemmas.
